kind inference

Core/Typing.lean
@@ -79,7 +79,7 @@ inductive Typing (G : List Global) : List Kind -> List Ty -> Term -> Ty -> Prop
   ctor_count dt G = some (n + 1) ->   -- need to also have that n + 1 = length of ctors of R
   (∀ i pat B A,
     ps.indexOf pat = some i -> -- i is the index of the i-th pattern
-    ctor_ty pat G = some B ->
+    ctor_ty pat G = some B -> -- It has some type B
     StableTypeMatch Δ B R -> -- B has the same result type. i.e. B = ∀[K] X -> ... -> R
     PrefixTypeMatch Δ A B T -> -- the case type A and constructor type B have the same prefixes
     Typing G Δ Γ (cs i) A) ->
