Core/Algorithm/Kind.lean
@@ -1,0 +1,48 @@
+import Core.Ty
+import Core.Global
+
+def wf_kind : (K : Kind) -> Option Unit
+| ★ => return ()
+| ◯ => return ()
+| .arrow k1 k2 => do
+  _ <- wf_kind k1
+  _ <- wf_kind k2
+  return ()
+
+def Kind.is_arrow : (K : Kind) -> Option (Kind × Kind)
+| .arrow k1 k2 => return (k1 , k2)
+| _ => none
+
+
+def infer_kind (G : List Global) (Δ : List Kind) : Ty -> Option Kind
+| t#x => do
+  let T <- Δ[x]?
+  let _ <- wf_kind T
+  return T
+| gt#x => do
+  let T <- lookup_kind G x
+  let _ <- wf_kind T
+  return T
+| .arrow b t1 t2 => do
+  let k1 <- infer_kind G Δ t1
+  let _ <- wf_kind k1
+  let k2 <- infer_kind G Δ t2
+  let _ <- wf_kind k2
+  return .base b
+| .all K t => do
+  let _ <- wf_kind K
+  let tk <- infer_kind G (K :: Δ) t
+  let _ <- wf_kind tk
+  return ★
+| .eq K A B => do
+  let _ <- wf_kind K
+  let Ak <- infer_kind G Δ A
+  let Bk <- infer_kind G Δ B
+  if Ak == Bk && Ak == K then return ★ else none
+| .app A B => do
+  let Ak <- infer_kind G Δ A
+  let _ <- wf_kind Ak
+  let Bk <- infer_kind G Δ B
+  let _ <- wf_kind Bk
+  let (k1, k2) <- Ak.is_arrow
+  if k1 == Bk then return k2 else none
