Core/Algorithm/Type.lean
@@ -1,0 +1,8 @@
+import Core.Ty
+import Core.Algorithm.Kind
+import Core.Global
+
+def infer_type (G : List Global) (Δ : List Kind) (Γ : List Ty) : Term -> Option Ty
+| #x =>  Γ[x]?
+| g#x => lookup_type G x
+| _ => sorry
